more

_lessons/dafny/abstract-queue.dfy
@@ -4,16 +4,16 @@
 
 class Queue<T> {
   // Abtract representation of the queue's elements
-  ghost var Content: seq<T>;
+  ghost var Content: seq<T>
 
   // Concrete implementation of the queue
   // container for the queue's elements
-  var a: array<T>;
+  var a: array<T>
   // size of the queue
-  var n: nat;
+  var n: nat
 
-  predicate Valid()
-  reads this, a;
+  ghost predicate Valid()
+  reads this, a
   {
     // Concrete class invariant
     n <= a.Length &&
@@ -24,9 +24,9 @@ class Queue<T> {
   }
 
   constructor (d: T)
-    ensures Valid();
-    ensures fresh(a);
-    ensures Content == [];
+    ensures Valid()
+    ensures fresh(a)
+    ensures Content == []
   {
     a := new T[5](_ => d); // initializes every array element to d
     n := 0;
@@ -36,22 +36,22 @@ class Queue<T> {
   }
 
   method front() returns (e: T)
-    requires Valid();
-    requires Content != [];
-    ensures Valid();
-    ensures Content == old(Content);
-    ensures e == Content[0];
+    requires Valid()
+    requires Content != []
+    ensures Valid()
+    ensures Content == old(Content)
+    ensures e == Content[0]
   {
     e := a[0];
   }
 
   method enqueue(e: T)
-    modifies this, a;
-    requires Valid();
-    ensures Valid();
-    ensures old(n) < old(a.Length) ==> a == old(a);
-    ensures old(n) == old(a.Length) ==> fresh(a);
-    ensures Content == old(Content) + [e];
+    modifies this, a
+    requires Valid()
+    ensures Valid()
+    ensures old(n) < old(a.Length) ==> a == old(a)
+    ensures old(n) == old(a.Length) ==> fresh(a)
+    ensures Content == old(Content) + [e]
   {
     if (n == a.Length) {
       var b := new T[2 * a.Length](_ => e);
@@ -68,13 +68,13 @@ class Queue<T> {
   }
 
   method dequeue() returns (e: T)
-    modifies this, a;
-    requires Content != [];
-    requires Valid();
-    ensures Valid();
-    ensures a == old(a);
-    ensures Content == old(Content[1..]);
-    ensures [e] + Content == old(Content);
+    modifies this, a
+    requires Content != []
+    requires Valid()
+    ensures Valid()
+    ensures a == old(a)
+    ensures Content == old(Content[1..])
+    ensures [e] + Content == old(Content)
   {
     e := a[0];
     n := n - 1;
@@ -88,17 +88,17 @@ class Queue<T> {
 }
 method Main ()
 {
-  var q := new Queue<int>(0);  assert q.Content == [];
-  q.enqueue(1);                assert q.Content == [1];
-  q.enqueue(2);                assert q.Content == [1,2];
-  q.enqueue(3);                assert q.Content == [1,2,3];
-  q.enqueue(2);                assert q.Content == [1,2,3,2];
-  q.enqueue(4);                assert q.Content == [1,2,3,2,4];
+  var q := new Queue<int>(0);  //assert q.Content == [];
+  q.enqueue(1);                //assert q.Content == [1];
+  q.enqueue(2);                //assert q.Content == [1,2];
+  q.enqueue(3);                //assert q.Content == [1,2,3];
+  q.enqueue(2);                //assert q.Content == [1,2,3,2];
+  q.enqueue(4);                //assert q.Content == [1,2,3,2,4];
 
-  var f := q.front();          assert f == 1 && q.a[..q.n] == [1,2,3,2,4];
+  var f := q.front();          //assert f == 1 && q.a[..q.n] == [1,2,3,2,4];
   print "Front of the list is ", f, "\n";
-  f := q.dequeue();            assert           q.Content == [2,3,2,4];
-  q.enqueue(5);                assert           q.Content == [2,3,2,4,5];
+  f := q.dequeue();            //assert           q.Content == [2,3,2,4];
+  q.enqueue(5);                //assert           q.Content == [2,3,2,4,5];
   f := q.front();
   print "Now front of the list is ", f, "\n";
 }
